\documentclass{article}

\usepackage{amsmath}
\usepackage{amssymb}

\begin{document}
\begin{align*}
  \lambda A x &= x\\
  x'x &= I\\
\end{align*}
\begin{align*}
  \frac{\partial \lambda}{\partial p}Ax + \lambda\frac{\partial
  A}{\partial p}x + \lambda A\frac{\partial x}{\partial p} &=
                                                            \frac{\partial x}{\partial p}\\
  \left(\frac{\partial x}{\partial p}\right)' x +
  x'\frac{\partial x}{\partial p} &= 0 \\
   x'\left( \frac{\partial \lambda}{\partial p}Ax + \lambda\frac{\partial
  A}{\partial p}x + \lambda A\frac{\partial x}{\partial p}\right) &+\\
  \left(\frac{\partial \lambda}{\partial p}Ax + \lambda\frac{\partial
  A}{\partial p}x + \lambda A\frac{\partial x}{\partial p}\right)'x &= 0
\end{align*}
\end{document}
